DAO/Rocq/Unravel/ocaml/unravel.mli
@@ -1,0 +1,181 @@
+
+val add : int -> int -> int
+
+val mul : int -> int -> int
+
+val sub : int -> int -> int
+
+module Nat :
+ sig
+  val sub : int -> int -> int
+
+  val leb : int -> int -> bool
+
+  val divmod : int -> int -> int -> int -> int*int
+
+  val div : int -> int -> int
+
+  val modulo : int -> int -> int
+ end
+
+val eqb : string -> string -> bool
+
+module UnravelLang :
+ sig
+  module Core :
+   sig
+    type coq_Expr =
+    | ENum of int
+    | EVoid
+    | EBool of bool
+    | EAdd of coq_Expr * coq_Expr
+    | ESub of coq_Expr * coq_Expr
+    | EMul of coq_Expr * coq_Expr
+    | EDiv of coq_Expr * coq_Expr
+    | EMod of coq_Expr * coq_Expr
+    | EIsVoid of coq_Expr
+    | EIfVoid of coq_Expr * coq_Expr * coq_Expr
+    | EDefault of coq_Expr * coq_Expr
+
+    type coq_Value =
+    | VNum of int
+    | VBool of bool
+    | VVoid
+
+    val is_void : coq_Value -> bool
+
+    val value_to_nat_default : coq_Value -> int -> int
+
+    val value_to_bool_default : coq_Value -> bool -> bool
+   end
+
+  module Eval :
+   sig
+    val eval : int -> Core.coq_Expr -> Core.coq_Value
+
+    val eval_default : Core.coq_Expr -> Core.coq_Value
+   end
+
+  module WithVariables :
+   sig
+    type coq_ExprV =
+    | EVNum of int
+    | EVVoid
+    | EVBool of bool
+    | EVAdd of coq_ExprV * coq_ExprV
+    | EVSub of coq_ExprV * coq_ExprV
+    | EVMul of coq_ExprV * coq_ExprV
+    | EVDiv of coq_ExprV * coq_ExprV
+    | EVMod of coq_ExprV * coq_ExprV
+    | EVIsVoid of coq_ExprV
+    | EVIfVoid of coq_ExprV * coq_ExprV * coq_ExprV
+    | EVDefault of coq_ExprV * coq_ExprV
+    | EVVar of string
+    | EVLet of string * coq_ExprV * coq_ExprV
+
+    type coq_Env = (string*Core.coq_Value) list
+
+    val lookup : coq_Env -> string -> Core.coq_Value
+
+    val evalV : int -> coq_Env -> coq_ExprV -> Core.coq_Value
+
+    val evalV_empty : coq_ExprV -> Core.coq_Value
+
+    module VariableExamples :
+     sig
+      val simple_let : coq_ExprV
+
+      val nested_let : coq_ExprV
+
+      val undefined_var : coq_ExprV
+
+      val void_binding : coq_ExprV
+
+      val shadowing : coq_ExprV
+
+      val recover_undefined : coq_ExprV
+
+      val complex_with_vars : coq_ExprV
+     end
+   end
+
+  module ThermodynamicUnravelLang :
+   sig
+    type coq_VoidInfo =
+    | VInfo of int * int * coq_VoidSource
+    and coq_VoidSource =
+    | DivByZero of int
+    | ModByZero of int
+    | UndefinedVar of string
+    | OutOfFuel
+    | TypeError of string
+    | VoidPropagation of coq_VoidInfo * coq_VoidInfo
+
+    type coq_ValueT =
+    | VTNum of int
+    | VTBool of bool
+    | VTVoid of coq_VoidInfo
+
+    type coq_Universe = { total_entropy : int; time_step : int;
+                          void_count : int }
+
+    val total_entropy : coq_Universe -> int
+
+    val time_step : coq_Universe -> int
+
+    val void_count : coq_Universe -> int
+
+    val initial_universe : coq_Universe
+
+    val evolve_universe : coq_Universe -> coq_VoidInfo -> coq_Universe
+
+    val combine_voids :
+      coq_VoidInfo -> coq_VoidInfo -> coq_Universe -> coq_VoidInfo
+
+    val lookupT : (string*coq_ValueT) list -> string -> coq_ValueT option
+
+    val evalT :
+      int -> coq_Universe -> (string*coq_ValueT) list ->
+      WithVariables.coq_ExprV -> coq_ValueT*coq_Universe
+
+    val evalT_initial : WithVariables.coq_ExprV -> coq_ValueT*coq_Universe
+
+    val value_entropy : coq_ValueT -> int
+
+    val is_heat_death : coq_Universe -> bool
+   end
+
+  module Examples :
+   sig
+    val safe_div : int -> int -> Core.coq_Expr
+
+    val divides : int -> int -> Core.coq_Expr
+
+    val calculation : Core.coq_Expr
+
+    val risky_calculation : Core.coq_Expr
+
+    val recovered : Core.coq_Expr
+   end
+
+  module ExtractionOcaml :
+   sig
+    val chaos_generator : int -> WithVariables.coq_ExprV
+
+    module Runner :
+     sig
+      val test_simple : Core.coq_Value
+
+      val test_void : Core.coq_Value
+
+      val test_recovery : Core.coq_Value
+
+      val test_let : Core.coq_Value
+
+      val test_thermo :
+        ThermodynamicUnravelLang.coq_ValueT*ThermodynamicUnravelLang.coq_Universe
+
+      val get_entropy : WithVariables.coq_ExprV -> int
+     end
+   end
+ end
